Reformat code to make use of Mac Malone's argument style code.

InfinitePrimes.lean
@@ -1,3 +1,33 @@
+/- Bullet format code by Mac Malone -/
+import Lean.Parser.Term
+open Lean
+open Parser.Term
+
+/-- A bullet argument: A nameable argument with sugar for functions. -/
+syntax bulletArg := atomic(ident funBinder* (typeSpec)? " := ")? term
+
+/-- Provide a number of arguments as an indented bulleted list. -/
+syntax:lead term:max " ⇐ " ppIndent(many1Indent(ppLine "· " bulletArg)) : term
+
+macro_rules
+  | `(term| $e ⇐ $[· $as]*) =>
+    as.foldlM (β := Term) (init := e) fun e a =>
+      match a with
+      | `(bulletArg| $id:ident $bs* $[$ty?]? :=%$dtk $a) =>
+        if bs.size > 0 then
+          `($e ($id :=%$dtk fun $bs* $[$ty?]? => $a))
+        else
+          if let some ty := ty? then
+            match ty with
+            | `(typeSpec| :%$tk $ty) =>
+              `($e ($id :=%$dtk ($a :%$tk $ty)))
+            | _ => Macro.throwErrorAt ty "ill-formed type specifier"
+          else
+            `($e ($id :=%$dtk $a))
+      | `(bulletArg| $a:term) => `($e $a)
+      | _ => Macro.throwErrorAt a "ill-formed bullet argument"
+/- End bullet format code -/
+
 variable {a b : Nat}
 
 def divides (n m : Nat) : Prop :=
@@ -7,74 +37,91 @@ local notation n " ∣ " m => divides n m
 local notation n " ∤ " m => ¬ (n ∣ m)
 
 abbrev Reg (n : Nat) :=
-  2 ≤ n 
+  2 ≤ n
 
 abbrev RegularRange (r n : Nat) :=
-  2 ≤ r ∧ r < n
+  (2 ≤ r) ∧ (r < n)
 
 local infix:50 " ⋖ " => RegularRange
 
-abbrev pos_of_nz : x ≠ 0 → 0 < x :=
+abbrev pos_of_nz : (x ≠ 0) → (0 < x) :=
   Nat.zero_lt_of_ne_zero
 
-abbrev nz_of_pos : 0 < x → x ≠ 0 :=
+abbrev nz_of_pos : (0 < x) → (x ≠ 0) :=
   Nat.not_eq_zero_of_lt
 
 def Prime (k : Nat) :=
-  Reg k ∧ ∀ n m : Nat, (k ∣ n * m) → (k ∣ n) ∨ (k ∣ m)
+  (Reg k) ∧ ∀ n m : Nat, (k ∣ n * m) → (k ∣ n) ∨ (k ∣ m)
 
 def NatPrime (k : Nat) :=
-  Reg k ∧ ∀ m, 2 ≤ m ∧ m < k → (m ∤ k)
+  (Reg k) ∧ ∀ m, (2 ≤ m) ∧ (m < k) → (m ∤ k)
 
-theorem eq_of_le_of_not_lt (h1 : a ≤ b) (h2 : ¬ a < b) :
+theorem eq_of_le_of_not_lt (h₁ : a ≤ b) (h₂ : ¬ a < b) :
     a = b :=
-  Nat.le_antisymm h1 (Nat.ge_of_not_lt h2)
+  Nat.le_antisymm ⇐
+  · h₁
+  · Nat.ge_of_not_lt h₂
 
-theorem eq_of_lt_succ_of_not_lt (h1 : a < b + 1) (h2 : ¬ a < b) :
+theorem eq_of_lt_succ_of_not_lt (h₁ : a < b + 1) (h₂ : ¬ a < b) :
     a = b :=
-  Nat.le_antisymm
-    (Nat.le_of_lt_succ h1)
-    (Nat.ge_of_not_lt  h2)
+  Nat.le_antisymm ⇐
+  · Nat.le_of_lt_succ h₁
+  · Nat.ge_of_not_lt  h₂
 
 def decidableForallInRange (p : Nat → Prop) [DecidablePred p] (b n : Nat) :
-    Decidable (∀ k, b ≤ k ∧ k < n → p k) :=
+    Decidable <| ∀ k, (b ≤ k) ∧ (k < n) → (p k) :=
   if n_le_b : n ≤ b then
-    isTrue <| fun k ⟨lower, upper⟩ =>
-    False.elim <| Nat.lt_irrefl n <| calc
-      n ≤ b := n_le_b
-      _ ≤ k := lower
-      _ < n := upper 
+    isTrue <|
+    fun k ⟨lower, upper⟩ =>
+      False.elim      <|
+      Nat.lt_irrefl n <|
+      calc
+        n ≤ b := n_le_b
+        _ ≤ k := lower
+        _ < n := upper
   else
     let m := n - 1
     have b_lt_n : b < n :=
       Nat.gt_of_not_le n_le_b
     have succ_m : n = m + 1 :=
-      Nat.not_eq_zero_of_lt b_lt_n |> Nat.succ_pred |>.symm
-    have b_le_m : b ≤ m := Nat.le_of_lt_succ <|
+      Nat.not_eq_zero_of_lt b_lt_n
+      |> Nat.succ_pred
+      |>.symm
+    have b_le_m : b ≤ m :=
+      Nat.le_of_lt_succ <|
       Nat.succ_eq_add_one m ▸ succ_m ▸ b_lt_n
     match decidableForallInRange p b m with
-    | isFalse not_forall_to_m => isFalse <|
+    | isFalse not_forall_to_m =>
+      isFalse <|
       fun forall_to_succ_m =>
-      have forall_to_m :
-      ∀ k, b ≤ k ∧ k < m → p k :=
-        fun k ⟨b_le_k, k_lt_m⟩ =>
-        have : k < m + 1 :=
-          Nat.lt_trans k_lt_m (Nat.lt_succ_self m)
-        forall_to_succ_m k ⟨b_le_k, succ_m ▸ this⟩
-      not_forall_to_m forall_to_m
+        have forall_to_m :
+        ∀ k, (b ≤ k) ∧ (k < m) → (p k) :=
+          fun k ⟨b_le_k, k_lt_m⟩ =>
+          have : k < m + 1 :=
+            Nat.lt_trans ⇐
+            · k_lt_m
+            · Nat.lt_succ_self m
+          forall_to_succ_m k ⟨b_le_k, succ_m ▸ this⟩
+        not_forall_to_m forall_to_m
     | isTrue forall_to_m =>
-      if p_m : p m then
-        isTrue  <| fun k ⟨b_le_k, k_lt_succ_m⟩ =>
+      if m_satisfies_p? : p m then
+        isTrue <|
+        fun k ⟨b_le_k, k_lt_succ_m⟩ =>
           if k_lt_m : k < m then
             forall_to_m k ⟨b_le_k, k_lt_m⟩
           else
-            have : k = m :=
-              eq_of_lt_succ_of_not_lt
-                (succ_m ▸ k_lt_succ_m) k_lt_m
-            this ▸ p_m
+            have k_eq_m : k = m :=
+              eq_of_lt_succ_of_not_lt ⇐
+              · succ_m ▸ k_lt_succ_m
+              · k_lt_m
+            k_eq_m ▸ m_satisfies_p?
       else
-        isFalse <| fun forall_to_succ_m =>
-          p_m <| forall_to_succ_m m ⟨b_le_m, succ_m ▸ Nat.lt_succ_self m⟩
+        isFalse <|
+        fun forall_to_succ_m =>
+          m_satisfies_p? <|
+          forall_to_succ_m ⇐
+          · m
+          · ⟨b_le_m, succ_m ▸ Nat.lt_succ_self m⟩
 
 theorem double_neg_elim [Decidable p] :
     (¬ (¬ p)) → p :=
@@ -84,51 +131,64 @@ theorem double_neg_elim [Decidable p] :
     (. hp |>.elim)
 
 theorem or_of_left (or_pred: p ∨ q) (proof : p → q) : q :=
-  Or.elim or_pred proof id
+  Or.elim ⇐
+  · or_pred
+  · proof
+  · id
 
 theorem or_of_right (or_pred: q ∨ p) (proof : p → q) : q :=
-  Or.elim or_pred id proof
+  Or.elim ⇐
+  · or_pred
+  · id
+  · proof
 
-notation orp " >l " pr => or_of_left orp pr
-notation orp " >r " pr => or_of_right orp pr
+local notation orp " ↗ " pr => or_of_left orp pr
+local notation orp " ↘ " pr => or_of_right orp pr
 
-def minSatRec [DecidablePred p] (r : Nat) (r_le_n : r ≤ n)
-    (witness : p n) (sofar : ∀ k, k < r → ¬ p k) :
-    ∃ m, p m ∧ ∀ k, k < m → ¬ p k :=
-  if succ_r_le_n : r + 1 ≤ n then 
+def minSatRec [DecidablePred p] (r : Nat) (r_le_n : r ≤ n) (witness : p n) (sofar : ∀ k, (k < r) → (¬ p k)) :
+    ∃ m, (p m) ∧ ∀ k, (k < m) → (¬ p k) :=
+  if succ_r_le_n : r + 1 ≤ n then
     if stop : p r then
       ⟨r, stop, sofar⟩
     else
-      have recursive_arg :
-      (k : Nat) → k < (r + 1) → ¬ p k :=
+      have recursive : (k : Nat) → k < (r + 1) → (¬ p k) :=
         fun k k_lt_succ =>
-        if already : k < r then
-          sofar k already
-        else
-          have equality : k = r :=
-            eq_of_le_of_not_lt
-              (Nat.le_of_lt_succ k_lt_succ)
-              already
-          equality ▸ stop
-      minSatRec (r + 1) succ_r_le_n witness recursive_arg
+          if already : k < r then
+            sofar k already
+          else
+            have equality : k = r :=
+              eq_of_le_of_not_lt ⇐
+              · Nat.le_of_lt_succ k_lt_succ
+              · already
+            equality ▸ stop
+      minSatRec ⇐
+      · r + 1
+      · succ_r_le_n
+      · witness
+      · recursive
   else
-    have : r = n :=
-      eq_of_le_of_not_lt r_le_n succ_r_le_n
-    ⟨n, witness, this ▸ sofar⟩
+    have r_eq_n : r = n :=
+      eq_of_le_of_not_lt ⇐
+      · r_le_n
+      · succ_r_le_n
+    ⟨n, witness, r_eq_n ▸ sofar⟩
 termination_by _ => n - r
 
 def minimal_satisfies {n : Nat} [DecidablePred p] (witness : p n) :
-    ∃ m, p m ∧ (∀ k, k < m → ¬ p k) := 
-  minSatRec 0
-    (Nat.zero_le n)
-    witness
-    (Nat.not_lt_zero . . |>.elim)  
+    ∃ m, (p m) ∧ ∀ k, (k < m) → (¬ p k) :=
+  minSatRec ⇐
+  · 0
+  · Nat.zero_le n
+  · witness
+  · (Nat.not_lt_zero . . |>.elim)
 
-theorem pos_of_reg : Reg n → n > 0 :=
-  (Nat.lt_trans (Nat.zero_lt_of_ne_zero Nat.one_ne_zero) .)
+theorem pos_of_reg  (reg_n : Reg n) : n > 0 :=
+  Nat.lt_trans ⇐
+  · Nat.zero_lt_of_ne_zero Nat.one_ne_zero
+  · reg_n
 
-theorem nz_of_reg : Reg n → n ≠ 0 :=
-  (Nat.not_eq_zero_of_lt .)
+theorem nz_of_reg (reg_n : Reg n) : n ≠ 0 :=
+  Nat.not_eq_zero_of_lt reg_n
 
 theorem pred_ge_one_of_reg (reg_d : Reg d) : 1 ≤ d - 1 :=
   Nat.pred_le_pred reg_d
@@ -137,19 +197,24 @@ theorem reg_monotone (reg_k : Reg k) (mono : k ≤ l) : Reg l :=
   Nat.le_trans reg_k mono
 
 theorem pred_lt_of_reg (reg_d : Reg d) : d - 1 < d :=
-  pos_of_reg reg_d |> Nat.not_eq_zero_of_lt |> Nat.pred_lt
+  pos_of_reg reg_d
+  |> Nat.not_eq_zero_of_lt
+  |> Nat.pred_lt
 
 theorem reg_pred_of_reg_ne_two (reg_d : Reg d) (ne : d ≠ 2) :
     Reg (d - 1) :=
-  Nat.pred_le_pred <| Nat.lt_of_le_of_ne reg_d ne.symm
+  Nat.pred_le_pred <|
+  Nat.lt_of_le_of_ne ⇐
+  · reg_d
+  · ne.symm
 
-theorem reg_of_mul_regs (rx: Reg x) (ry :Reg y) : Reg (x * y) :=
-  calc 2 ≤ 4     := by decide 
-       _ ≤ x * y := Nat.mul_le_mul rx ry
+theorem reg_of_mul_regs (rx: Reg x) (ry :Reg y) : Reg (x * y) := calc
+  2 ≤ 4     := by decide
+  _ ≤ x * y := Nat.mul_le_mul rx ry
 
-theorem zero_one_of_not_reg (nreg_d : ¬ Reg d) :
-    d = 0 ∨ d = 1 :=
-  have : d < 2 := Nat.gt_of_not_le nreg_d
+theorem zero_one_of_not_reg (nreg_d : ¬ Reg d) : (d = 0) ∨ (d = 1) :=
+  have : d < 2 :=
+    Nat.gt_of_not_le nreg_d
   match d with
   | 0 => .inl rfl
   | 1 => .inr rfl
@@ -158,50 +223,62 @@ abbrev reg_by_match (k : Nat) :=
   Nat.add_comm 2 k ▸ Nat.le_add_right 2 k
 
 theorem eq_of_sandwich {a x : Nat} (ax: a ≤ x) (xa : x ≤ a) :
-    a = x :=
-  calc a = (a - x) + x := Nat.sub_add_cancel xa |>.symm
-       _ = x           := by rw [Nat.sub_eq_zero_of_le ax, Nat.zero_add]
+    a = x := calc
+  a = (a - x) + x := Nat.sub_add_cancel xa |>.symm
+  _ = x           := by rw [Nat.sub_eq_zero_of_le ax, Nat.zero_add]
 
 theorem mod_cancel_prod (n d q : Nat) :
     (q * d + n) % d = n % d :=
   match q with
   | 0     => by rw [Nat.zero_mul, Nat.zero_add]
   | q + 1 => by
-    rw [Nat.right_distrib, Nat.one_mul,
-        Nat.add_assoc, Nat.add_comm d n, ← Nat.add_assoc]
-    have : q * d + n + d ≥ d := Nat.le_add_left d _
-    rw [Nat.mod_eq_sub_mod this, Nat.add_sub_assoc,
-        Nat.sub_self, Nat.add_zero]
+    rw [ Nat.right_distrib ,
+         Nat.one_mul       ,
+         Nat.add_assoc     ,
+         Nat.add_comm d n  ,
+         ← Nat.add_assoc   ]
+    have : q * d + n + d ≥ d :=
+      Nat.le_add_left d _
+    rw [ Nat.mod_eq_sub_mod this ,
+         Nat.add_sub_assoc       ,
+         Nat.sub_self            ,
+         Nat.add_zero            ]
     exact mod_cancel_prod n d q
     exact Nat.le_refl d
 
 theorem euclidean_data (d_pos : 0 < d) (n_pos : 0 < n) :
-    (r < d ∧ n = q * d + r) ↔ (r = n % d ∧ q = n / d) :=
-  have div_mod := Nat.div_add_mod n d
-  ⟨ fun ⟨r_lt_d, ediv⟩ => 
+    (r < d) ∧ (n = q * d + r) ↔ (r = n % d) ∧ (q = n / d) :=
+  have div_mod :=
+    Nat.div_add_mod n d
+  Iff.intro ⇐
+  · fun ⟨r_lt_d, ediv⟩ =>
       have rem_id : r = n % d := calc
         r = r % d           := Nat.mod_eq_of_lt r_lt_d |>.symm
         _ = (q * d + r) % d := mod_cancel_prod r d q   |>.symm
         _ = n % d           := ediv ▸ rfl
-      ⟨ rem_id,
-        have : d * (n / d) + r = n := rem_id.symm ▸ div_mod
+      And.intro ⇐
+      · rem_id
+      · have : d * (n / d) + r = n :=
+          rem_id.symm ▸ div_mod
         have : d * (n / d) = d * q := calc
           d * (n / d) = d * (n / d) + r - r := by rw [Nat.add_sub_cancel]
           _           = n - r               := by rw [this]
-          _           = d * q               := by rw [ediv, Nat.add_sub_cancel,
-                                                      Nat.mul_comm]
-        Nat.eq_of_mul_eq_mul_left d_pos this.symm ⟩,
-    fun ⟨r_eq_mod, q_eq_div⟩ =>
-      ⟨ r_eq_mod ▸ Nat.mod_lt n d_pos,
-        have := r_eq_mod.symm ▸ q_eq_div.symm ▸ div_mod
-        by rw [Nat.mul_comm, this]⟩⟩
+          _           = d * q               := by rw [ ediv               ,
+                                                       Nat.add_sub_cancel ,
+                                                       Nat.mul_comm       ]
+        Nat.eq_of_mul_eq_mul_left d_pos this.symm
+  · fun ⟨r_eq_mod, q_eq_div⟩ =>
+      And.intro ⇐
+      · r_eq_mod ▸ Nat.mod_lt n d_pos
+      · have := r_eq_mod.symm ▸ q_eq_div.symm ▸ div_mod
+        by rw [Nat.mul_comm, this]
 
 theorem euclidean_division (d_pos : 0 < d) (n_pos : 0 < n) :
     ∃ q r, r < d ∧ n = q*d + r :=
-  ⟨n / d, n % d, by
-    rw [euclidean_data d_pos n_pos]; apply And.intro <;> rfl⟩
+  ⟨ (n / d), (n % d),
+    (by rw [euclidean_data d_pos n_pos]; apply And.intro <;> rfl) ⟩
 
-theorem le_or_zero_of_dvd (k K : Nat) :
+theorem zero_or_le_of_dvd (k K : Nat) :
     (k ∣ K) → K = 0 ∨ k ≤ K :=
   fun ⟨m, kdiv⟩ =>
     if mz : m = 0 then
@@ -215,22 +292,22 @@ theorem le_or_zero_of_dvd (k K : Nat) :
 theorem not_lt_of_dvd_pos (k_pos : 0 < K) :
     (k ∣ K) → ¬ K < k :=
   fun divs contra =>
-  le_or_zero_of_dvd k K divs |>.elim
-    (fun kzr => Nat.ne_of_lt k_pos kzr.symm)
-    (fun kle => Nat.not_le_of_gt contra kle)
+    (zero_or_le_of_dvd k K divs |>.elim) ⇐
+    · fun kzr => Nat.ne_of_lt k_pos kzr.symm
+    · fun kle => Nat.not_le_of_gt contra kle
 
 theorem le_of_dvd_pos (k_pos : 0 < K) (dk : k ∣ K) :
     k ≤ K :=
-  le_or_zero_of_dvd k K dk >l
+  zero_or_le_of_dvd k K dk ↗
     (. |> nz_of_pos k_pos |>.elim)
 
-theorem one_of_dvd_one : (a ∣ 1) → a = 1 :=
-  fun ⟨k, ka_eq_one⟩ =>
+theorem one_of_dvd_one (a_div_one : a ∣ 1) : a = 1 :=
+  let ⟨k, ka_eq_one⟩ := a_div_one
   have a_pos : a ≥ 1 :=
-    Nat.eq_zero_or_pos _ >l
+    Nat.eq_zero_or_pos _ ↗
       fun _ => by simp only [*, Nat.mul_zero]
   have k_pos : k ≥ 1 :=
-    Nat.eq_zero_or_pos _ >l
+    Nat.eq_zero_or_pos _ ↗
       fun _ => by simp only [*, Nat.zero_mul]
   have : a ≤ 1 := calc
     a = 1 * a := Nat.one_mul a |>.symm
@@ -243,7 +320,8 @@ theorem dvd_zero (a : Nat) : a ∣ 0 :=
 
 theorem zero_of_dvd_by_zero :
     ∀ (a : Nat), (0 ∣ a) → a = 0 :=
-  fun _ ⟨k, h⟩ => (Nat.mul_zero k) ▸ h
+  fun _ ⟨k, h⟩ =>
+    Nat.mul_zero k ▸ h
 
 theorem dvd_transAux :
     (a ∣ b) ∧ (b ∣ c) → (a ∣ c) :=
@@ -260,13 +338,14 @@ theorem dvd_diff_of_both : (a ∣ b) ∧ (a ∣ c) → (a ∣ b - c) :=
   fun ⟨⟨m, adb⟩, ⟨n, bdc⟩⟩ =>
     ⟨m - n, by rw [adb, bdc, Nat.mul_sub_right_distrib]⟩
 
-theorem dvd_monotone (r : Nat) (div : p ∣ q) :
+theorem dvd_monotone (r : Nat) (p_dvd_q : p ∣ q) :
     p ∣ q * r :=
-  have : q ∣ q * r := ⟨r, by rw [Nat.mul_comm]⟩
-  dvd_trans div this
+  have q_dvd_qr : q ∣ q * r :=
+    ⟨r, by rw [Nat.mul_comm]⟩
+  dvd_trans p_dvd_q q_dvd_qr
 
-theorem dvd_of_eq : a = r → a ∣ r :=
-  fun _ => ⟨1, by simp only [*, Nat.one_mul]⟩
+theorem dvd_of_eq (a_eq_r : a = r) : a ∣ r :=
+  ⟨1, by simp only [*, Nat.one_mul]⟩
 
 theorem dvd_self : n ∣ n :=
   ⟨1, by rw [Nat.one_mul]⟩
@@ -275,42 +354,51 @@ theorem zmod_of_dvd (n m : Nat) : (n ∣ m) → m % n = 0 :=
   if m_zero : m = 0 then
     fun _ => by rw [m_zero, Nat.zero_mod]
   else if n_zero : n = 0 then
-    (n_zero ▸ . |> zero_of_dvd_by_zero m |> m_zero |>.elim)
+    ( n_zero ▸ . |> zero_of_dvd_by_zero m |> m_zero |>.elim )
   else if big_n : m < n then
-    (le_or_zero_of_dvd n m . |>.elim
-      (m_zero . |>.elim)
-      (Nat.not_le_of_gt big_n . |>.elim))
+    ( zero_or_le_of_dvd n m . |>.elim
+        ( m_zero . |>.elim )
+        ( Nat.not_le_of_gt big_n . |>.elim ) )
   else if eq_n : n = m then
     fun _ => eq_n ▸ Nat.mod_self n
   else
-    have small_n : n ≤ m := Nat.ge_of_not_lt big_n
+    have small_n : n ≤ m :=
+      Nat.ge_of_not_lt big_n
     fun n_div_m =>
-    have := zmod_of_dvd n (m - n) <|
-            dvd_diff_of_both ⟨n_div_m, dvd_self⟩
-    this ▸ Nat.mod_eq_sub_mod small_n
+      have sub_zero :=
+        zmod_of_dvd n (m - n) <|
+        dvd_diff_of_both ⟨n_div_m, dvd_self⟩
+      sub_zero ▸ Nat.mod_eq_sub_mod small_n
 decreasing_by
-  simp_wf; exact Nat.sub_lt
-    (Nat.zero_lt_of_ne_zero m_zero)
-    (Nat.zero_lt_of_ne_zero n_zero)
+  exact Nat.sub_lt ⇐
+  · Nat.zero_lt_of_ne_zero m_zero
+  · Nat.zero_lt_of_ne_zero n_zero
 
 theorem dvd_of_zmod (n m : Nat) : m % n = 0 → (n ∣ m) :=
   fun mod_z =>
-  have : n * (m / n) = m :=
-    Nat.add_zero (n * (m / n)) ▸ mod_z ▸ Nat.div_add_mod m n
-  ⟨m / n, by rw [Nat.mul_comm, this]⟩
+    have cancel_n : n * (m / n) = m :=
+      Nat.add_zero (n * (m / n)) ▸ mod_z ▸
+      Nat.div_add_mod m n
+    ⟨m / n, by rw [Nat.mul_comm, cancel_n]⟩
 
 theorem div_self_eq_one (nz : a ≠ 0) : a / a = 1 :=
   have : a * (a / a) = a :=
-    Nat.add_zero (a * (a / a)) ▸ Nat.mod_self a ▸ Nat.div_add_mod a a
-  have cancel : a * (a / a) = a * 1 := by
+    Nat.add_zero (a * (a / a)) ▸
+    Nat.mod_self a ▸
+    Nat.div_add_mod a a
+  have cancel_a : a * (a / a) = a * 1 := by
     rw [Nat.mul_one, this]
-  Nat.eq_of_mul_eq_mul_left (pos_of_nz nz) cancel
+  Nat.eq_of_mul_eq_mul_left ⇐
+  · pos_of_nz nz
+  · cancel_a
 
 theorem expand_product {n m : Nat} (nx : n = a*x + p) (mx : m = a*y + q) :
   n * m = a*(x*a*y + x*q + p*y) + p*q := by
     rw [nx, mx]
-    simp only [Nat.add_assoc, Nat.left_distrib,
-               Nat.right_distrib, Nat.mul_assoc]
+    simp only [ Nat.add_assoc     ,
+                Nat.left_distrib  ,
+                Nat.right_distrib ,
+                Nat.mul_assoc     ]
     simp only [← Nat.add_assoc]
     have : p * (a * y) = a * (p * y) := calc
       p * (a * y) = (p * a) * y := by rw [Nat.mul_assoc]
@@ -321,16 +409,21 @@ theorem expand_product {n m : Nat} (nx : n = a*x + p) (mx : m = a*y + q) :
 
 def decDiv (n m : Nat) : Decidable (divides n m) :=
   if mod_zero : m % n = 0 then
-    isTrue  <| dvd_of_zmod n m mod_zero
+    isTrue  ⇐
+    · dvd_of_zmod n m mod_zero
   else
-    isFalse <| (zmod_of_dvd n m . |> mod_zero)
+    isFalse ⇐
+    · (zmod_of_dvd n m . |> mod_zero)
 
 instance : Decidable (divides n m) :=
   decDiv n m
 
 def decidableForallInRegRange (n : Nat) :
     Decidable (∀ k, k ⋖ n → k ∤ n) :=
-  decidableForallInRange (. ∤ n) 2 n
+  decidableForallInRange ⇐
+  · (. ∤ n)
+  · 2
+  · n
 
 instance : Decidable (NatPrime n) := by
   unfold NatPrime
@@ -339,81 +432,100 @@ instance : Decidable (NatPrime n) := by
 
 theorem prod_mod_eq_mod_prod_mod (d_pos : 0 < d) :
     (n * m) % d = (n % d)*(m % d) % d :=
-  if nz : n = 0 then
-    by rw [nz, Nat.zero_mul, Nat.zero_mod, Nat.zero_mul, Nat.zero_mod]
-  else if mz : m = 0 then
-    by rw [mz, Nat.mul_zero, Nat.zero_mod, Nat.mul_zero, Nat.zero_mod]
+  if nz : n = 0 then by
+    rw [ nz           ,
+         Nat.zero_mul ,
+         Nat.zero_mod ,
+         Nat.zero_mul ,
+         Nat.zero_mod ]
+  else if mz : m = 0 then by
+    rw [ mz           ,
+         Nat.mul_zero ,
+         Nat.zero_mod ,
+         Nat.mul_zero ,
+         Nat.zero_mod ]
   else
-    have np := pos_of_nz nz
-    have mp := pos_of_nz mz
-    have ⟨qn, rn, n_div⟩ := euclidean_division d_pos np
-    have ⟨qm, rm, m_div⟩ := euclidean_division d_pos mp
-    have div_n : n = d * qn + rn := by rw [Nat.mul_comm, n_div.2]
-    have div_m : m = d * qm + rm := by rw [Nat.mul_comm, m_div.2]
-    have mod_m_r := euclidean_data d_pos mp |>.mp m_div |>.left
-    have mod_n_r := euclidean_data d_pos np |>.mp n_div |>.left
+    have np : 0 < n := pos_of_nz nz
+    have mp : 0 < m := pos_of_nz mz
+    let ⟨qn, rn, n_div⟩ := euclidean_division d_pos np
+    let ⟨qm, rm, m_div⟩ := euclidean_division d_pos mp
+    have div_n   : n = (d * qn) + rn := by rw [Nat.mul_comm, n_div.2]
+    have div_m   : m = (d * qm) + rm := by rw [Nat.mul_comm, m_div.2]
+    have mod_m_r : rm = m % d := euclidean_data d_pos mp |>.mp m_div |>.left
+    have mod_n_r : rn = n % d := euclidean_data d_pos np |>.mp n_div |>.left
     have exp := expand_product div_n div_m
-    let f := qn * d * qm + qn * rm + rn * qm
+    let f := (qn * d * qm) + (qn * rm) + (rn * qm)
     calc
       (n * m) % d = (f * d + rn * rm) % d := by rw [exp, Nat.mul_comm]
-      _           = rn * rm % d           := by rw [mod_cancel_prod]
+      _           = (rn * rm) % d         := by rw [mod_cancel_prod]
       _           = (n % d) * (m % d) % d := by rw [mod_m_r, mod_n_r]
 
 theorem prime_of_not_dvd_prod (reg_n : Reg n)
-    (not_dvd_prod :
-      ∀ p q, 1 ≤ p ∧ p < n ∧ 1 ≤ q ∧ q < n → (n ∤ (p * q))) :
+    (not_dvd_prod : ∀ p q, (1 ≤ p) ∧ (p < n) ∧ (1 ≤ q) ∧ (q < n) → (n ∤ (p * q))) :
     Prime n :=
-  ⟨reg_n,
-    fun k l n_div_kl =>
-    let p := k % n
-    let q := l % n
-    have n_pos  : 0 < n := pos_of_reg reg_n
-    have p_lt_n : p < n := Nat.mod_lt k n_pos
-    have q_lt_n : q < n := Nat.mod_lt l n_pos
-    have n_div_pq : n ∣ (p * q) :=
-      dvd_of_zmod n (p * q) <| Eq.symm <| calc
-        0 = k * l % n           := zmod_of_dvd n (k * l) n_div_kl |>.symm
-        _ = (k % n)*(l % n) % n := prod_mod_eq_mod_prod_mod n_pos
-    if pos_p : 1 ≤ p then
-      if pos_q : 1 ≤ q then
-         not_dvd_prod p q ⟨pos_p, p_lt_n, pos_q, q_lt_n⟩ n_div_pq |>.elim
+  And.intro ⇐
+  · reg_n
+  · fun k l n_div_kl =>
+      let p := k % n
+      let q := l % n
+      have n_pos  : 0 < n := pos_of_reg reg_n
+      have p_lt_n : p < n := Nat.mod_lt k n_pos
+      have q_lt_n : q < n := Nat.mod_lt l n_pos
+      have n_div_pq : n ∣ (p * q) :=
+        dvd_of_zmod n (p * q) <| calc
+          p * q % n = k * l % n := prod_mod_eq_mod_prod_mod n_pos |>.symm
+          _         = 0         := zmod_of_dvd n (k * l) n_div_kl
+      if pos_p : 1 ≤ p then
+        if pos_q : 1 ≤ q then
+          n_div_pq
+          |> not_dvd_prod p q ⟨pos_p, p_lt_n, pos_q, q_lt_n⟩
+          |> False.elim
+        else
+          .inr            <|
+          dvd_of_zmod n l <|
+          Nat.eq_zero_or_pos q ↘
+            (pos_q . |>.elim)
       else
-        .inr <| dvd_of_zmod n l <| Nat.eq_zero_or_pos q >r (pos_q . |>.elim)
-    else
-      .inl <| dvd_of_zmod n k <| Nat.eq_zero_or_pos p >r (pos_p . |>.elim)⟩
+        .inl            <|
+        dvd_of_zmod n k <|
+        Nat.eq_zero_or_pos p ↘
+          (pos_p . |>.elim)
 
 theorem reduced_primality : Prime n →
     Reg n ∧ ∀ p q, p < n ∧ q < n → (n ∣ (p * q)) → (n ∣ p) ∨ (n ∣ q) :=
-  fun ⟨reg_n, div⟩ => ⟨reg_n, fun p q _ => div p q⟩
+  fun ⟨reg_n, div⟩ =>
+    ⟨reg_n, fun p q _ => div p q⟩
 
-def factors_of_dvd (dn : d ∣ n) : n = d * (n / d) :=
-  calc n = d * (n / d) + n % d := Nat.div_add_mod n d |>.symm
-       _ = d * (n / d)         := by rw [zmod_of_dvd d n dn, Nat.add_zero]
+def factors_of_dvd (dn : d ∣ n) : n = d * (n / d) := calc
+  n = d * (n / d) + n % d := Nat.div_add_mod n d |>.symm
+  _ = d * (n / d)         := by rw [ zmod_of_dvd d n dn ,
+                                     Nat.add_zero       ]
 
-theorem descend_factors
-    (d_pos : 0 < d) (div_p : d ∣ p) (div_c : d ∣ c)
-    (factor : p * q = c * n) :
+theorem descend_factors (d_pos : 0 < d) (div_p : d ∣ p) (div_c : d ∣ c) (factor : p * q = c * n) :
     (p / d) * q = (c / d) * n := by
-  rw [factors_of_dvd div_p, factors_of_dvd div_c] at factor
+  rw [ factors_of_dvd div_p ,
+       factors_of_dvd div_c ] at factor
   repeat rw [Nat.mul_assoc] at factor
   exact Nat.eq_of_mul_eq_mul_left d_pos factor
 
-theorem pos_of_div : 0 < d ∧ d ≤ n → 1 ≤ n / d :=
-  fun _ =>
+theorem pos_of_div (_ : 0 < d) (_ : d ≤ n) : 1 ≤ n / d :=
   have : n / d = (n - d)/d + 1 := by
-    rw [Nat.div_eq, if_pos]; assumption
-  calc 1 ≤ (n - d) / d + 1 := Nat.succ_le_succ <| Nat.zero_le _
-       _ = n / d           := this.symm
+    rw [Nat.div_eq, if_pos]
+    apply And.intro
+    repeat assumption
+  calc
+    1 ≤ (n - d) / d + 1 := Nat.succ_le_succ <| Nat.zero_le _
+    _ = n / d           := this.symm
 
 def MinDivisor (n d : Nat) : Prop :=
-  Reg d ∧ (d ∣ n) ∧ ∀ k, k ⋖ d → k ∤ n
+  (Reg d) ∧ (d ∣ n) ∧ ∀ k, (k ⋖ d) → (k ∤ n)
 
 def AuxMinDiv (n d : Nat) :
-    Decidable (∀ k, k ⋖ d → k ∤ n) :=
+    Decidable <| ∀ k, (k ⋖ d) → (k ∤ n) :=
   decidableForallInRange (. ∤ n) 2 d
 
 def decMinDivisor (n d : Nat) :
-    Decidable (MinDivisor n d) := by
+    Decidable <| MinDivisor n d := by
   unfold MinDivisor
   have := AuxMinDiv n d
   exact instDecidableAnd
@@ -422,49 +534,68 @@ instance : Decidable (MinDivisor n d) :=
   decMinDivisor n d
 
 abbrev AuxDivPred (n d : Nat) :=
-  Reg d ∧ (d ∣ n)
+  (Reg d) ∧ (d ∣ n)
 
-instance : Decidable (AuxDivPred n k) :=
+instance : Decidable <| AuxDivPred n k :=
   instDecidableAnd
 
-theorem neg_AuxDivPred : ¬ AuxDivPred n d ↔ ¬ Reg d ∨ d ∤ n :=
-  Decidable.not_and_iff_or_not (Reg d) (d ∣ n)
+theorem neg_AuxDivPred : (¬ AuxDivPred n d) ↔ (¬ Reg d) ∨ (d ∤ n) :=
+  Decidable.not_and_iff_or_not ⇐
+  · Reg d
+  · d ∣ n
 
 def hasMinDivisor (n : Nat) (reg_n : Reg n) :
-    ∃ d : Nat, MinDivisor n d :=
-  let self_sat : AuxDivPred n n := ⟨reg_n, dvd_self⟩
-  have minimal_sat := minimal_satisfies self_sat
+    ∃ d, MinDivisor n d :=
+  let self_sat : AuxDivPred n n :=
+    ⟨reg_n, dvd_self⟩
+  have minimal_sat :=
+    minimal_satisfies self_sat
   let ⟨d, ⟨reg_d, d_div_n⟩, no_smaller⟩ := minimal_sat
-  ⟨d, ⟨reg_d, d_div_n, 
-    fun k ⟨reg_k, k_lt_d⟩ =>
-    (no_smaller k k_lt_d |> neg_AuxDivPred.mp) >l
-      (. reg_k |>.elim) ⟩⟩
+  Exists.intro ⇐
+  · d
+  · And.intro ⇐
+    · reg_d
+    · And.intro ⇐
+      · d_div_n
+      · fun k ⟨reg_k, k_lt_d⟩ =>
+          (no_smaller k k_lt_d |> neg_AuxDivPred.mp) ↗
+            (. reg_k |>.elim)
 
 theorem NatPrime_of_MinDivisor : MinDivisor n p → NatPrime p :=
   fun ⟨reg_p, p_div_n, p_ndiv_rest⟩ =>
-  ⟨reg_p, fun k ⟨reg_k, k_lt_p⟩ div =>
-    have k_div_n : k ∣ n := dvd_trans div p_div_n
-    p_ndiv_rest k ⟨reg_k, k_lt_p⟩ k_div_n⟩
+    And.intro ⇐
+    · reg_p
+    · fun k ⟨reg_k, k_lt_p⟩ div =>
+        have k_div_n : k ∣ n :=
+          dvd_trans div p_div_n
+        p_ndiv_rest k ⟨reg_k, k_lt_p⟩ k_div_n
 
 theorem nat_prime_divisor :
     ∀ n, Reg n → ∃ p, NatPrime p ∧ (p ∣ n) :=
   fun n reg_n =>
-  have ⟨d, minDiv⟩ := hasMinDivisor n reg_n
-  ⟨d, NatPrime_of_MinDivisor minDiv, minDiv.2.1⟩
+    have ⟨d, minDiv⟩ :=
+      hasMinDivisor n reg_n
+    Exists.intro ⇐
+    · d
+    · And.intro ⇐
+     · NatPrime_of_MinDivisor minDiv
+     · minDiv.2.1
 
-theorem nat_of_prime : Prime n → NatPrime n :=
-  fun prime_n =>
-    let ⟨reg_n, red_prime⟩ := reduced_primality prime_n
-    ⟨reg_n,
-      fun d₁ ⟨reg₁, small₁⟩ small_div_n =>
-        let d₂ := n / d₁
-        have pos_d₁ : d₁ > 0 := pos_of_reg reg₁
-        have pos_d₂ : d₂ > 0 := pos_of_div ⟨pos_d₁, Nat.le_of_lt small₁⟩
-        have small₂ : d₂ < n := Nat.div_lt_self (pos_of_reg reg_n) reg₁
-        have : n = d₁ * d₂   := factors_of_dvd small_div_n
-        dvd_of_eq this |> red_prime d₁ d₂ ⟨small₁, small₂⟩ |>.elim
-          (fun div₁ => not_lt_of_dvd_pos pos_d₁ div₁ small₁)
-          (fun div₂ => not_lt_of_dvd_pos pos_d₂ div₂ small₂)⟩
+theorem nat_of_prime (prime_n : Prime n) : NatPrime n :=
+  let ⟨reg_n, red_prime⟩ :=
+    reduced_primality prime_n
+  And.intro ⇐
+  · reg_n
+  · fun d₁ ⟨reg₁, small₁⟩ small_div_n =>
+      let d₂ := n / d₁
+      have pos_d₁ : d₁ > 0      := pos_of_reg reg₁
+      have pos_d₂ : d₂ > 0      := pos_of_div pos_d₁ (Nat.le_of_lt small₁)
+      have small₂ : d₂ < n      := Nat.div_lt_self (pos_of_reg reg_n) reg₁
+      have factor : n = d₁ * d₂ := factors_of_dvd small_div_n
+      Or.elim ⇐
+      · dvd_of_eq factor |> red_prime d₁ d₂ ⟨small₁, small₂⟩
+      · fun div₁ => not_lt_of_dvd_pos pos_d₁ div₁ small₁
+      · fun div₂ => not_lt_of_dvd_pos pos_d₂ div₂ small₂
 
 theorem first_nat_prime : NatPrime 2 := by
   decide
@@ -478,27 +609,33 @@ theorem not_factor (factors : p = c * n) (small_p : p < n) (pos_c : 0 < c) :
     _ < n     := small_p
 
 def ReducibleDividend (n m : Nat) :=
-  (n ∣ m) ∧ ∃ p q, p ⋖ n ∧ q ⋖ n ∧ m = p * q
+  (n ∣ m) ∧ ∃ p q, (p ⋖ n) ∧ (q ⋖ n) ∧ (m = p * q)
 
 def decidable_exists (d : Nat → Nat → Prop) (n : Nat) [DecidablePred (d n)] :
-    Decidable (∃ p, p ⋖ n ∧ (d n p)) :=
+    Decidable <| ∃ p, (p ⋖ n) ∧ (d n p) :=
   if small_n : n ≤ 2 then
-    isFalse <| fun ⟨p, p_regular_range, _⟩ =>
-    Nat.lt_irrefl 2 <| calc
-      2 ≤ p := p_regular_range.1
-      _ < n := p_regular_range.2
-      _ ≤ 2 := small_n
-  else
-    have big_n : 2 < n := Nat.gt_of_not_le small_n
-    have : ¬ ∃ p, p ⋖ 2 ∧ d n p :=
-      fun ⟨p, contra, _⟩ =>
+    isFalse <|
+    fun ⟨p, p_regular_range, _⟩ =>
       Nat.lt_irrefl 2 <| calc
-        2 ≤ p := contra.1
-        _ < 2 := contra.2 
-    go 2 (by decide) (Nat.le_of_lt big_n) this where
-    go (k : Nat) (reg_k : Reg k) (k_le_n : k ≤ n)
-       (sofar : ¬ ∃ p, p ⋖ k ∧ (d n p)) :
-        Decidable  (∃ p, p ⋖ n ∧ (d n p)) :=
+        2 ≤ p := p_regular_range.1
+        _ < n := p_regular_range.2
+        _ ≤ 2 := small_n
+  else
+    have big_n : 2 < n :=
+      Nat.gt_of_not_le small_n
+    have initial_step : ¬ ∃ p, (p ⋖ 2) ∧ (d n p) :=
+      fun ⟨p, contra, _⟩ =>
+        Nat.lt_irrefl 2 <| calc
+          2 ≤ p := contra.1
+          _ < 2 := contra.2
+    descend ⇐
+    · 2
+    · by decide
+    · Nat.le_of_lt big_n
+    · initial_step
+    where
+    descend (k : Nat) (reg_k : Reg k) (k_le_n : k ≤ n) (sofar : ¬ ∃ p, (p ⋖ k) ∧ (d n p)) :
+        Decidable <| ∃ p, (p ⋖ n) ∧ (d n p) :=
       if k_eq_n : k = n then
         isFalse <| k_eq_n ▸ sofar
       else
@@ -508,24 +645,35 @@ def decidable_exists (d : Nat → Nat → Prop) (n : Nat) [DecidablePred (d n)] 
         if contra : d n k then
           isTrue ⟨k, reg_to, contra⟩
         else
-          have nextfar : ¬ ∃ p, p ⋖ (k + 1) ∧ (d n p) :=
+          have nextfar : ¬ ∃ p, (p ⋖ k + 1) ∧ (d n p) :=
             fun ⟨p, p_regular_range, p_sat⟩ =>
-            if p_lt_k : p < k then
-              have : p ⋖ k := ⟨p_regular_range.1, p_lt_k⟩
-              sofar ⟨p, this, p_sat⟩
-            else
-              have : p = k := eq_of_le_of_not_lt 
-                (Nat.le_of_lt_succ p_regular_range.2) p_lt_k
-              contra (this ▸ p_sat)
-          have _ : n - (k + 1) < n - k := Nat.sub_lt
-            (Nat.sub_ne_zero_of_lt k_lt_n |> Nat.zero_lt_of_ne_zero)
-            (Nat.zero_lt_succ 0)
-          have : k ≤ k + 1 := Nat.le_succ k 
-          go (k + 1) (reg_monotone reg_k this) succ_k_le_n nextfar 
+              if p_lt_k : p < k then
+                have : p ⋖ k :=
+                  ⟨p_regular_range.1, p_lt_k⟩
+                sofar ⟨p, this, p_sat⟩
+              else
+                have : p = k :=
+                  eq_of_le_of_not_lt ⇐
+                  · Nat.le_of_lt_succ p_regular_range.2
+                  · p_lt_k
+                contra <| this ▸ p_sat
+          have _ : n - (k + 1) < n - k :=
+            Nat.sub_lt ⇐
+            · Nat.sub_ne_zero_of_lt k_lt_n
+              |> Nat.zero_lt_of_ne_zero
+            · Nat.zero_lt_succ 0
+          have : k ≤ k + 1 :=
+            Nat.le_succ k
+          descend ⇐
+          · k + 1
+          · reg_monotone reg_k this
+          · succ_k_le_n
+          · nextfar
 termination_by
-  go _ => n - k
+  descend _ => n - k
 
-def divisionEq (n p q c : Nat) := p * q = c * n
+def divisionEq (n p q c : Nat) :=
+  p * q = c * n
 
 instance : Decidable (divisionEq n p q c) := by
   unfold divisionEq
@@ -533,179 +681,259 @@ instance : Decidable (divisionEq n p q c) := by
 
 def decidable_divisionEq (n q c : Nat) :
     Decidable (∃ p, p ⋖ n ∧ divisionEq n p q c) :=
-  decidable_exists (fun n x => divisionEq n x q c) n
+  decidable_exists ⇐
+  · fun n x => divisionEq n x q c
+  · n
 
 abbrev divisionPred (n q c : Nat) :=
-  ∃ p, p ⋖ n ∧ divisionEq n p q c
+  ∃ p, (p ⋖ n) ∧ (divisionEq n p q c)
 
-def decidable_div_pred : Decidable (divisionPred n q c) := by
+def decidable_div_pred : Decidable <| divisionPred n q c := by
   unfold divisionPred
   apply decidable_divisionEq
 
-instance : Decidable (divisionPred n q c) :=
+instance : Decidable <| divisionPred n q c :=
   decidable_div_pred
 
 def dec_ref (n c : Nat) :
-    Decidable (∃ q, q ⋖ n ∧ divisionPred n q c) :=
-  decidable_exists (fun n x => divisionPred n x c) n
+    Decidable <| ∃ q, (q ⋖ n) ∧ (divisionPred n q c) :=
+  decidable_exists ⇐
+  · fun n x => divisionPred n x c
+  · n
 
 abbrev divPred (n c : Nat) :=
-  ∃ q, q ⋖ n ∧ divisionPred n q c
+  ∃ q, (q ⋖ n) ∧ (divisionPred n q c)
 
-instance : Decidable (divPred n c) := by
+instance : Decidable <| divPred n c := by
   unfold divPred
   apply dec_ref
 
 def factorPredicate (n c : Nat) :=
   ∃ p q : Nat,
-    2 ≤ p ∧ p < n ∧
-    2 ≤ q ∧ q < n ∧
-    p * q = c * n
+    (2 ≤ p) ∧ (p < n) ∧
+    (2 ≤ q) ∧ (q < n) ∧
+    (p * q = c * n)
 
 theorem factorPredicate_iff_divPred :
     divPred n c ↔ factorPredicate n c :=
-  ⟨fun h => by
-    unfold divPred divisionPred divisionEq RegularRange at h
-    have ⟨q, ⟨⟨reg_q, q_lt_n⟩, p, ⟨reg_p, p_lt_n⟩, eq⟩⟩ := h
-    unfold factorPredicate
-    exact ⟨p, q, reg_p, p_lt_n, reg_q, q_lt_n, eq⟩,
-  fun h => by
-    unfold factorPredicate at h
-    have ⟨p, q, reg_p, p_lt_n, reg_q, q_lt_n, eq⟩ := h
-    unfold divPred divisionPred divisionEq RegularRange
-    exact ⟨q, ⟨⟨reg_q, q_lt_n⟩, p, ⟨reg_p, p_lt_n⟩, eq⟩⟩⟩
+  Iff.intro ⇐
+  · fun h => by
+      unfold divPred divisionPred divisionEq RegularRange at h
+      have ⟨q, ⟨⟨reg_q, q_lt_n⟩, p, ⟨reg_p, p_lt_n⟩, eq⟩⟩ := h
+      unfold factorPredicate
+      exact ⟨p, q, reg_p, p_lt_n, reg_q, q_lt_n, eq⟩
+  · fun h => by
+      unfold factorPredicate at h
+      have ⟨p, q, reg_p, p_lt_n, reg_q, q_lt_n, eq⟩ := h
+      unfold divPred divisionPred divisionEq RegularRange
+      exact ⟨q, ⟨⟨reg_q, q_lt_n⟩, p, ⟨reg_p, p_lt_n⟩, eq⟩⟩
 
-instance : Decidable (factorPredicate n c) :=
+instance : Decidable <| factorPredicate n c :=
   if h : divPred n c then
-    isTrue  <| factorPredicate_iff_divPred.mp h
+    isTrue  <|
+    factorPredicate_iff_divPred.mp h
   else
-    isFalse <| fun contra => h <| factorPredicate_iff_divPred.mpr contra
+    isFalse <|
+    (h <| factorPredicate_iff_divPred.mpr .)
 
-abbrev Factors {n : Nat} (c : Nat) := factorPredicate n c
+abbrev Factors {n : Nat} (c : Nat) :=
+  factorPredicate n c
 
 mutual
-theorem reduced_predicate : NatPrime n → 
-    ∀ p q, 1 ≤ p ∧ p < n ∧ 1 ≤ q ∧ q < n → (n ∤ (p * q)) :=
-  fun nat_prime_n p q ⟨pos_p, p_lt_n, pos_q, q_lt_n⟩ =>
-  have reg_n : Reg n := nat_prime_n.1
-  if      pz : p = 0 then have := pz ▸ pos_p; by contradiction
-  else if qz : q = 0 then have := qz ▸ pos_q; by contradiction
-  else if po : p = 1 then fun n_div_pq =>
-    have := Nat.one_mul q ▸ po ▸ n_div_pq
-    have := le_of_dvd_pos pos_q <| this
-    Nat.lt_irrefl q <| calc
-      q < n := q_lt_n
-      _ ≤ q := this
-  else if qo : q = 1 then fun n_div_pq =>
-    have := Nat.mul_one p ▸ qo ▸ n_div_pq
-    have := le_of_dvd_pos pos_p <| this
-    Nat.lt_irrefl p <| calc
-      p < n := p_lt_n
-      _ ≤ p := this
-  else
-    have reg_p : Reg p := match p with | k + 2 => reg_by_match k
-    have reg_q : Reg q := match q with | k + 2 => reg_by_match k
-    fun ⟨c, pq_eq_nc⟩ =>
-      have some_sat : Factors c :=
-        ⟨p, q, reg_p, p_lt_n, reg_q, q_lt_n, pq_eq_nc⟩
-      have minimal : ∃ m, Factors m ∧ (∀ k, k < m → ¬ Factors k) :=
-        minimal_satisfies some_sat
-      let ⟨m, ⟨rs_eq_mn, no_smaller⟩⟩ := minimal
-      if mz : m = 0 then by
-        unfold Factors factorPredicate at rs_eq_mn
-        let ⟨p, q, ⟨reg_p, _, reg_q, _, pq_eq_mn⟩⟩ := rs_eq_mn
-        rw [mz, Nat.zero_mul] at pq_eq_mn
-        have := reg_of_mul_regs reg_p reg_q
-        exact nz_of_reg this pq_eq_mn
-      else if mo : m = 1 then by
-        unfold Factors factorPredicate at rs_eq_mn
-        let ⟨p, q, ⟨reg_p, p_lt_n, _, _, pq_eq_mn⟩⟩ := rs_eq_mn
-        rw [mo, Nat.one_mul] at pq_eq_mn
-        have : p ∣ n := ⟨q, by rw [Nat.mul_comm, pq_eq_mn.symm]⟩
-        have : p ∤ n := nat_prime_n.2 p ⟨reg_p, p_lt_n⟩
-        contradiction
-      else
-        have reg_m : Reg m := match m with | k + 2 => reg_by_match k 
-        let ⟨p, q, ⟨reg_p, p_lt_n, reg_q, q_lt_n, pq_eq_mn⟩⟩ := rs_eq_mn
-        have : n * m < n * q := calc
-          n * m = m * n := Nat.mul_comm n m
-          _     = p * q := pq_eq_mn.symm
-          _     < n * q := Nat.mul_lt_mul_of_pos_right p_lt_n (pos_of_reg reg_q)
-        have m_lt_n : m < n := calc
-          m ≤ q := Nat.le_of_mul_le_mul_left (Nat.le_of_lt this) (pos_of_reg reg_n)
-          _ < n := q_lt_n
-        let ⟨p₀, nat_prime_po, po_div_m⟩ := nat_prime_divisor m reg_m
-        have : p₀ < n := calc
-          p₀ ≤ m := le_of_dvd_pos (pos_of_reg reg_m) po_div_m
-          _  < n := m_lt_n
-        have pq_eq_nm : p * q = n * m := Nat.mul_comm n m ▸ pq_eq_mn
-        have prime_o : Prime p₀ := prime_of_nat <| nat_prime_po
-        have : (p₀ ∣ p) ∨ (p₀ ∣ q) := prime_o.2 p q <|
-          dvd_trans po_div_m ⟨n, pq_eq_nm⟩
-        this.elim (
-          fun po_div_p =>
-          have descent : (p / p₀) * q = n * (m / p₀) :=
-            have := descend_factors (pos_of_reg prime_o.1) po_div_p po_div_m  pq_eq_mn
-            Nat.mul_comm n (m / p₀) ▸ this
-          have po_lt_m : m / p₀ < m := Nat.div_lt_self (pos_of_reg reg_m) prime_o.1
-          if  reg_po : Reg (p / p₀) then
-            have po_lt_n : p / p₀ < n := Nat.lt_trans
-              (Nat.div_lt_self (pos_of_reg reg_p) (prime_o.1))
-              p_lt_n
-            have : @Factors n (m / p₀) :=
-              ⟨p / p₀, q, reg_po, po_lt_n, reg_q, q_lt_n,
-               Nat.mul_comm (m / p₀) n ▸ descent⟩
-            no_smaller (m / p₀) po_lt_m this |>.elim
-          else
-            zero_one_of_not_reg reg_po |>.elim
-              (fun x => pos_of_div ⟨pos_of_reg prime_o.1,
-                le_of_dvd_pos (pos_of_reg reg_p) po_div_p⟩ |>
-                Nat.not_eq_zero_of_lt <| x)
-              (fun po_one =>
-                have : q = (m / p₀) * n :=
-                  Nat.mul_comm (m / p₀) n ▸ Nat.one_mul q ▸ po_one ▸ descent
-                not_factor this q_lt_n (pos_of_div
-                  ⟨pos_of_reg prime_o.1,
-                  le_of_dvd_pos (pos_of_reg reg_m) po_div_m⟩) |>.elim)
-        ) (
-          fun po_div_q =>
-          have descent : (q / p₀) * p = n * (m / p₀) :=
-            have : q * p = m * n := Nat.mul_comm p q ▸ pq_eq_mn
-            have := descend_factors (pos_of_reg prime_o.1) po_div_q po_div_m  this
-            Nat.mul_comm n (m / p₀) ▸ this
-          have po_lt_m : m / p₀ < m := Nat.div_lt_self (pos_of_reg reg_m) prime_o.1
-          if reg_po : Reg (q / p₀) then
-            have po_lt_n : q / p₀ < n := Nat.lt_trans
-              (Nat.div_lt_self (pos_of_reg reg_q) (prime_o.1))
-              q_lt_n
-            have : @Factors n (m / p₀) :=
-              ⟨q / p₀, p, reg_po, po_lt_n, reg_p, p_lt_n,
-               Nat.mul_comm (m / p₀) n ▸ descent⟩
-            no_smaller (m / p₀) po_lt_m this |>.elim
-          else
-            zero_one_of_not_reg reg_po |>.elim
-              (fun x => pos_of_div ⟨pos_of_reg prime_o.1,
-                le_of_dvd_pos (pos_of_reg reg_q) po_div_q⟩ |>
-                Nat.not_eq_zero_of_lt <| x
-              )
-              (fun po_one =>
-                have : p = (m / p₀) * n :=
-                  Nat.mul_comm (m / p₀) n ▸ Nat.one_mul p ▸ po_one ▸ descent
-                not_factor this p_lt_n (pos_of_div
-                  ⟨pos_of_reg prime_o.1,
-                  le_of_dvd_pos (pos_of_reg reg_m) po_div_m⟩) |>.elim))
+theorem reduced_predicate : NatPrime n →
+    ∀ p q, (1 ≤ p) ∧ (p < n) ∧ (1 ≤ q) ∧ (q < n) → (n ∤ (p * q)) :=
+  fun nat_prime_n p q
+      ⟨pos_p, p_lt_n, pos_q, q_lt_n⟩ =>
+    have reg_n : Reg n :=
+      nat_prime_n.1
+    if      pz : p = 0 then have := pz ▸ pos_p; by contradiction
+    else if qz : q = 0 then have := qz ▸ pos_q; by contradiction
+    else if po : p = 1 then
+      fun n_div_pq =>
+        have := Nat.one_mul q ▸ po ▸ n_div_pq
+        have := le_of_dvd_pos pos_q <| this
+        Nat.lt_irrefl q <|
+        calc
+          q < n := q_lt_n
+          _ ≤ q := this
+    else if qo : q = 1 then
+      fun n_div_pq =>
+        have := Nat.mul_one p ▸ qo ▸ n_div_pq
+        have := le_of_dvd_pos pos_p <| this
+        Nat.lt_irrefl p <| calc
+          p < n := p_lt_n
+          _ ≤ p := this
+    else
+      have reg_p := match p with | k + 2 => reg_by_match k
+      have reg_q := match q with | k + 2 => reg_by_match k
+      fun ⟨c, pq_eq_nc⟩ =>
+        have some_sat : Factors c :=
+          ⟨p, q, reg_p, p_lt_n, reg_q, q_lt_n, pq_eq_nc⟩
+        have minimal : ∃ m, Factors m ∧ ∀ k, (k < m) → (¬ Factors k) :=
+          minimal_satisfies some_sat
+        let ⟨m, ⟨rs_eq_mn, no_smaller⟩⟩ := minimal
+        if mz : m = 0 then by
+          unfold Factors factorPredicate at rs_eq_mn
+          let ⟨p, q, ⟨reg_p, _, reg_q, _, pq_eq_mn⟩⟩ := rs_eq_mn
+          rw [mz, Nat.zero_mul] at pq_eq_mn
+          have := reg_of_mul_regs reg_p reg_q
+          exact nz_of_reg this pq_eq_mn
+        else if mo : m = 1 then by
+          unfold Factors factorPredicate at rs_eq_mn
+          let ⟨p, q, ⟨reg_p, p_lt_n, _, _, pq_eq_mn⟩⟩ := rs_eq_mn
+          rw [mo, Nat.one_mul] at pq_eq_mn
+          have : p ∣ n := ⟨q, by rw [Nat.mul_comm, pq_eq_mn.symm]⟩
+          have : p ∤ n := nat_prime_n.2 p ⟨reg_p, p_lt_n⟩
+          contradiction
+        else
+          have reg_m := match m with | k + 2 => reg_by_match k
+          let ⟨p, q, ⟨reg_p, p_lt_n, reg_q, q_lt_n, pq_eq_mn⟩⟩ := rs_eq_mn
+          have : n * m < n * q := calc
+            n * m = m * n := Nat.mul_comm n m
+            _     = p * q := pq_eq_mn.symm
+            _     < n * q := Nat.mul_lt_mul_of_pos_right ⇐
+                              · p_lt_n
+                              · pos_of_reg reg_q
+          have m_lt_n : m < n := calc
+            m ≤ q := Nat.le_of_mul_le_mul_left ⇐
+                      · Nat.le_of_lt this
+                      · pos_of_reg reg_n
+            _ < n := q_lt_n
+          let ⟨p₀, nat_prime_po, po_div_m⟩ := nat_prime_divisor m reg_m
+          have : p₀ < n := calc
+            p₀ ≤ m := le_of_dvd_pos (pos_of_reg reg_m) po_div_m
+            _  < n := m_lt_n
+          have pq_eq_nm : p * q = n * m :=
+            Nat.mul_comm n m ▸ pq_eq_mn
+          have prime_o : Prime p₀ :=
+            prime_of_nat <| nat_prime_po
+          have po_div_p_or_q : (p₀ ∣ p) ∨ (p₀ ∣ q) :=
+            prime_o.2 p q <|
+            dvd_trans ⇐
+            · po_div_m
+            · ⟨n, pq_eq_nm⟩
+          po_div_p_or_q.elim ⇐
+          · fun po_div_p =>
+              have descent : (p / p₀) * q = n * (m / p₀) :=
+                have aux_descent :=
+                  descend_factors ⇐
+                  · pos_of_reg prime_o.1
+                  · po_div_p
+                  · po_div_m
+                  · pq_eq_mn
+                Nat.mul_comm n (m / p₀) ▸ aux_descent
+              have po_lt_m : m / p₀ < m :=
+                Nat.div_lt_self ⇐
+                · pos_of_reg reg_m
+                · prime_o.1
+              if  reg_po : Reg (p / p₀) then
+                have po_lt_n : p / p₀ < n :=
+                  Nat.lt_trans ⇐
+                  · Nat.div_lt_self ⇐
+                    · pos_of_reg reg_p
+                    · prime_o.1
+                  · p_lt_n
+                have contra_minimal : @Factors n (m / p₀) :=
+                  ⟨ p / p₀, q,
+                    reg_po, po_lt_n,
+                    reg_q, q_lt_n,
+                    Nat.mul_comm (m / p₀) n ▸ descent ⟩
+                False.elim <|
+                  no_smaller ⇐
+                  · m / p₀
+                  · po_lt_m
+                  · contra_minimal
+              else
+                (zero_one_of_not_reg reg_po |>.elim) ⇐
+                · fun x =>
+                    (pos_of_div ⇐
+                    · pos_of_reg prime_o.1
+                    · le_of_dvd_pos ⇐
+                      · pos_of_reg reg_p
+                      · po_div_p)
+                    |> Nat.not_eq_zero_of_lt <| x
+                · fun po_one =>
+                    have : q = (m / p₀) * n :=
+                      Nat.mul_comm (m / p₀) n ▸ Nat.one_mul q ▸
+                      po_one ▸ descent
+                    not_factor ⇐
+                    · this
+                    · q_lt_n
+                    · pos_of_div ⇐
+                      · pos_of_reg prime_o.1
+                      · le_of_dvd_pos ⇐
+                        · pos_of_reg reg_m
+                        · po_div_m
+          · fun po_div_q =>
+            have descent : (q / p₀) * p = n * (m / p₀) :=
+              have : q * p = m * n :=
+                Nat.mul_comm p q ▸ pq_eq_mn
+              have aux_descent :=
+                descend_factors ⇐
+                · pos_of_reg prime_o.1
+                · po_div_q
+                · po_div_m
+                · this
+              Nat.mul_comm n (m / p₀) ▸ aux_descent
+            have po_lt_m : m / p₀ < m :=
+              Nat.div_lt_self ⇐
+              · pos_of_reg reg_m
+              · prime_o.1
+            if reg_po : Reg (q / p₀) then
+              have po_lt_n : q / p₀ < n :=
+                Nat.lt_trans ⇐
+                · Nat.div_lt_self ⇐
+                  · pos_of_reg reg_q
+                  · prime_o.1
+                · q_lt_n
+              have contra_minimal : @Factors n (m / p₀) :=
+                ⟨ q / p₀, p,
+                  reg_po, po_lt_n,
+                  reg_p, p_lt_n,
+                  Nat.mul_comm (m / p₀) n ▸ descent ⟩
+              False.elim <|
+                no_smaller ⇐
+                · (m / p₀)
+                · po_lt_m
+                · contra_minimal
+            else
+              Or.elim ⇐
+              · zero_one_of_not_reg reg_po
+              · fun po_zero =>
+                  (pos_of_div ⇐
+                  · pos_of_reg prime_o.1
+                  · le_of_dvd_pos ⇐
+                    · pos_of_reg reg_q
+                    · po_div_q)
+                  |> Nat.not_eq_zero_of_lt <| po_zero
+              · fun po_one =>
+                  have p_factor : p = (m / p₀) * n :=
+                    Nat.mul_comm (m / p₀) n ▸ Nat.one_mul p ▸
+                    po_one ▸ descent
+                  not_factor ⇐
+                  · p_factor
+                  · p_lt_n
+                  · pos_of_div ⇐
+                    · pos_of_reg prime_o.1
+                    · le_of_dvd_pos ⇐
+                      · pos_of_reg reg_m
+                      · po_div_m
 
 theorem prime_of_nat : NatPrime n → Prime n :=
   fun nat_prime_n =>
-  let ⟨reg_n, _⟩ := nat_prime_n
-  prime_of_not_dvd_prod reg_n <| reduced_predicate nat_prime_n
+    let ⟨reg_n, _⟩ := nat_prime_n
+    prime_of_not_dvd_prod ⇐
+    · reg_n
+    · reduced_predicate nat_prime_n
 end
 
-instance : Decidable (Prime n) :=
+instance : Decidable <| Prime n :=
   if h : NatPrime n then
-    isTrue  <| prime_of_nat h
+    isTrue  <|
+    prime_of_nat h
   else
-    isFalse <| (h <| nat_of_prime .)
+    isFalse <|
+    (h <| nat_of_prime .)
 
 theorem first_prime : Prime 2 := by
   decide
@@ -728,32 +956,43 @@ theorem dvd_fact (pos_k : 0 < k) (ineq : k ≤ n) :
         dvd_monotone (fact r) dvd_self
       assumption
     else
-      have : k ≤ r           := Nat.pred_le_pred <| Nat.lt_of_le_of_ne ineq h
-      have : k ∣ fact r := dvd_fact pos_k this
-      have k_dvd_product     := dvd_monotone (r + 1) this
+      have : k ≤ r       := Nat.pred_le_pred <| Nat.lt_of_le_of_ne ineq h
+      have : k ∣ fact r  := dvd_fact pos_k this
+      have k_dvd_product := dvd_monotone (r + 1) this
       by rw [Nat.mul_comm] at k_dvd_product; assumption
 
 theorem fact_positive : ∀ n, fact n > 0
   | 0     => by decide
-  | k + 1 => Nat.mul_pos (Nat.succ_pos k) (fact_positive k)
+  | k + 1 =>
+    Nat.mul_pos ⇐
+    · Nat.succ_pos k
+    · fact_positive k
 
 theorem unbounded_primes :
     ∀ n, ∃ p, Prime p ∧ p > n :=
   fun n =>
-  let Q := fact n + 1
-  have reg_q : Reg Q := 
-    Nat.add_le_add (fact_positive n) (Nat.le_refl 1)
-  let ⟨p, nat_prime_p, p_div_q⟩ := nat_prime_divisor Q reg_q
+  let Q := (fact n) + 1
+  have reg_q : Reg Q :=
+    Nat.add_le_add ⇐
+    · fact_positive n
+    · Nat.le_refl 1
+  let ⟨p, nat_prime_p, p_div_q⟩ :=
+    nat_prime_divisor Q reg_q
   have prime_p : Prime p :=
-    prime_of_nat <| nat_prime_p
+    prime_of_nat nat_prime_p
   if contra : p ≤ n then
-    have p_div_fact : p ∣ fact n :=
-      dvd_fact (pos_of_reg nat_prime_p.1) contra 
+    have p_div_fact : p ∣ (fact n) :=
+      dvd_fact ⇐
+      · pos_of_reg nat_prime_p.1
+      · contra
     have dvd_diff : p ∣ 1 := calc
       p ∣ (fact n + 1) - fact n := dvd_diff_of_both ⟨p_div_q, p_div_fact⟩
       _ = (1 + fact n) - fact n := by rw [Nat.add_comm]
-      _ = 1 := by simp only [Nat.add_sub_assoc, Nat.le_refl, Nat.sub_self] 
-    have : p = 1 := one_of_dvd_one dvd_diff
+      _ = 1                     := by simp only [ Nat.add_sub_assoc ,
+                                                  Nat.le_refl       ,
+                                                  Nat.sub_self      ]
+    have : p = 1 :=
+      one_of_dvd_one dvd_diff
     have := this ▸ nat_prime_p.1
     by contradiction
   else
